fixed LetE

Syntax.v
@@ -150,7 +150,7 @@ Section Phoas.
 
   Inductive LetExprSyntax k :=
   | NormExpr (e: Expr (SyntaxKind k)): LetExprSyntax k
-  | LetE k' (e: Expr (SyntaxKind k')) (cont: ty k' -> LetExprSyntax k): LetExprSyntax k.
+  | LetE k' (e: LetExprSyntax k') (cont: ty k' -> LetExprSyntax k): LetExprSyntax k.
 
   Section BitOps.
     Definition castBits ni no (pf: ni = no) (e: Expr (SyntaxKind (Bit ni))) :=
@@ -363,7 +363,7 @@ Section Phoas.
   Fixpoint convertLetExprSyntax_ActionT k (e: LetExprSyntax k) :=
     match e in LetExprSyntax _ return ActionT k with
     | NormExpr e' => Return e'
-    | LetE _ e' cont => LetExpr e' (fun v => convertLetExprSyntax_ActionT (cont v))
+    | LetE _ e' cont => LetAction (convertLetExprSyntax_ActionT e') (fun v => convertLetExprSyntax_ActionT (cont v))
     end.
 End Phoas.
 
@@ -1158,7 +1158,7 @@ Section Semantics.
   Fixpoint evalLetExpr k (e: LetExprSyntax type k) :=
     match e in LetExprSyntax _ _ return type k with
     | NormExpr e' => evalExpr e'
-    | LetE _ e' cont => evalLetExpr (cont (evalExpr e'))
+    | LetE _ e' cont => evalLetExpr (cont (evalLetExpr e'))
     end.
 
   Variable o: RegsT.
@@ -1444,10 +1444,20 @@ Section Semantics.
     destruct evalA; eauto; repeat eexists; try destruct (evalExpr p); eauto; try discriminate.
   Qed.
 
+  Lemma DisjKey_nils A B: @DisjKey A B nil nil.
+  Proof.
+    unfold DisjKey; intro.
+    left; simpl; auto.
+  Qed.
+  
   Lemma convertLetExprSyntax_ActionT_same k (e: LetExprSyntax type k):
     SemAction (convertLetExprSyntax_ActionT e) nil nil nil (evalLetExpr e).
   Proof.
-    induction e; simpl; constructor; auto.
+    induction e; simpl; try constructor; auto.
+    specialize (H (evalLetExpr e)).
+    pose proof (SemLetAction (fun v => convertLetExprSyntax_ActionT (cont v)) (@DisjKey_nils string _) IHe H) as sth.
+    rewrite ?(app_nil_l nil) in sth.
+    auto.
   Qed.
   
   Lemma SemActionReadsSub k a reads upds calls ret:
